src/bag/primeFactorScript.sml
@@ -1,0 +1,135 @@
+(*---------------------------------------------------------------------------*)
+(* Fundamental theorem of arithmetic for num.                                *)
+(*---------------------------------------------------------------------------*)
+
+open HolKernel Parse boolLib simpLib BasicProvers SingleStep metisLib
+     bagTheory dividesTheory arithmeticTheory;
+
+(* Interactive
+quietdec := true;
+app load ["dividesTheory", "gcdTheory", "bagTheory"];
+open dividesTheory bagTheory arithmeticTheory;
+quietdec := false;
+*)
+
+val _ = new_theory "primeFactor";
+
+infix ++;
+val std_ss =
+     (boolSimps.bool_ss ++ pairSimps.PAIR_ss ++ optionSimps.OPTION_ss ++
+      numSimps.REDUCE_ss ++ sumSimps.SUM_ss ++ combinSimps.COMBIN_ss ++
+      numSimps.ARITH_RWTS_ss);
+
+val arith_ss = std_ss ++ numSimps.ARITH_DP_ss
+val DECIDE = numLib.ARITH_PROVE;
+
+fun DECIDE_TAC (g as (asl,_)) =
+((MAP_EVERY UNDISCH_TAC (filter numSimps.is_arith_asm asl)
+      THEN numLib.ARITH_TAC)
+ ORELSE
+ tautLib.TAUT_TAC
+ ORELSE
+ NO_TAC) g;
+
+
+val MULT_LEFT_CANCEL = Q.prove
+(`!m n p. 0 < m ==> ((m*n = m*p) = (n=p))`,
+ Cases_on `m` THEN RW_TAC arith_ss []);
+
+val PRIME_FACTORS_EXIST = Q.store_thm
+("PRIME_FACTORS_EXIST",
+ `!n. 1 < n ==>
+        ?b. FINITE_BAG b /\ 
+            (!m. BAG_IN m b ==> prime m) /\
+            (n = BAG_GEN_PROD b 1)`,
+ completeInduct_on `n` THEN STRIP_TAC THEN Cases_on `prime n` THENL
+ [Q.EXISTS_TAC `{|n|}` THEN 
+    SRW_TAC [] [BAG_GEN_PROD_TAILREC,BAG_GEN_PROD_EMPTY],
+  `?m. prime m /\ divides m n` by RW_TAC arith_ss [PRIME_FACTOR] THEN
+  `?q. m * q = n` by METIS_TAC [divides_def,MULT_SYM] THEN 
+  `q < n` by
+     (STRIP_ASSUME_TAC (DECIDE ``q < n \/ (q=n) \/ n < q``) THENL
+      [FULL_SIMP_TAC arith_ss [MULT_EQ_ID] THEN METIS_TAC [NOT_PRIME_1],
+       `0 < m /\ 0 < q` by METIS_TAC [ZERO_LESS_MULT,DECIDE ``0 < 1``,LESS_TRANS] THEN
+       RW_TAC arith_ss [] THEN
+       `(m=1) \/ 1 < m` by DECIDE_TAC THEN METIS_TAC [NOT_PRIME_1]]) THEN
+  `1 < q` by 
+     (STRIP_ASSUME_TAC (DECIDE ``(q = 0) \/ (q=1) \/ 1 < q``) THEN 
+      RW_TAC arith_ss [] THEN METIS_TAC [MULT_RIGHT_1]) THEN
+  (* use IH *)
+  `?b. FINITE_BAG b /\ (!k. BAG_IN k b ==> prime k) /\
+       (q = BAG_GEN_PROD b 1)` by METIS_TAC [] THEN
+  Q.EXISTS_TAC `BAG_INSERT m b` THEN SRW_TAC [][] THENL 
+  [METIS_TAC [], METIS_TAC [], METIS_TAC [BAG_GEN_PROD_REC]]]);
+
+val PRIME_FACTORS_def = new_specification
+("PRIME_FACTORS_def",
+ ["PRIME_FACTORS"],
+ SIMP_RULE bool_ss [SKOLEM_THM,GSYM RIGHT_EXISTS_IMP_THM] PRIME_FACTORS_EXIST);
+
+val lem1 = Q.prove
+(`!b. FINITE_BAG b
+     ==> !m. prime m /\ 
+             divides m (BAG_GEN_PROD b 1) /\ 
+             (!x. BAG_IN x b ==> prime x)
+     ==> BAG_IN m b`,
+ HO_MATCH_MP_TAC STRONG_FINITE_BAG_INDUCT THEN REPEAT STRIP_TAC THENL
+ [FULL_SIMP_TAC arith_ss [BAG_GEN_PROD_EMPTY] THEN 
+    METIS_TAC [DIVIDES_ONE,NOT_PRIME_1],
+  Q.PAT_ASSUM `divides p q` MP_TAC THEN RW_TAC arith_ss [BAG_GEN_PROD_REC] THEN
+    METIS_TAC [gcdTheory.P_EUCLIDES,prime_divides_only_self,BAG_IN_BAG_INSERT]]);
+
+(*---------------------------------------------------------------------------*)
+(* Uniqueness.                                                               *)
+(* Sketch of the proof. When bag b1 is non-empty it has a prime p in it. We  *)
+(* can show p divides BAG_PROD b2, so p is also in b2 (because p is prime).  *)
+(* Let b1' = b1-p and b2' = b2-p. Then b1' = b2', by induction hypothesis.   *)
+(* Thus b1=b2. The argument uses a lemma derived from gcdTheory.P_EUCLIDES,  *)
+(* which says that p divides (a*b) ==> p divides a or p divides b.           *)
+(*---------------------------------------------------------------------------*)
+
+val UNIQUE_PRIME_FACTORS = store_thm
+("UNIQUE_PRIME_FACTORS",
+ ``!n b1 b2. 
+   (FINITE_BAG b1 /\ (!m. BAG_IN m b1 ==> prime m) /\ (n=BAG_GEN_PROD b1 1)) /\
+   (FINITE_BAG b2 /\ (!m. BAG_IN m b2 ==> prime m) /\ (n=BAG_GEN_PROD b2 1)) 
+    ==> (b1 = b2)``,
+completeInduct_on `n` THEN 
+ REPEAT STRIP_TAC THEN POP_ASSUM SUBST_ALL_TAC THEN 
+ `(b1 = {||}) \/ ?b1' e. b1 = BAG_INSERT e b1'` by METIS_TAC [BAG_cases] THENL
+ [RW_TAC arith_ss [] THEN 
+    STRIP_ASSUME_TAC (ISPEC ``b2:num bag`` BAG_cases) THEN 
+    FULL_SIMP_TAC arith_ss [] THEN RW_TAC std_ss [] THEN 
+    Q.PAT_ASSUM `BAG_GEN_PROD a b = BAG_GEN_PROD c d` MP_TAC THEN 
+    `FINITE_BAG b0` by METIS_TAC [FINITE_BAG_THM] THEN 
+    ASM_SIMP_TAC arith_ss [BAG_GEN_PROD_EMPTY,BAG_GEN_PROD_TAILREC] THEN 
+    STRIP_TAC THEN `e = 1` by METIS_TAC [BAG_GEN_PROD_EQ_1] THEN
+    METIS_TAC [BAG_GEN_PROD_ALL_ONES, NOT_PRIME_1, BAG_IN_BAG_INSERT],
+  `prime e` by METIS_TAC [BAG_IN_BAG_INSERT] THEN RW_TAC std_ss [] THEN 
+  `FINITE_BAG b1'` by METIS_TAC [FINITE_BAG_THM] THEN 
+ Q.PAT_ASSUM `p = q` MP_TAC THEN RW_TAC std_ss [BAG_GEN_PROD_REC] THEN 
+ `divides e (BAG_GEN_PROD b2 1)` by METIS_TAC [divides_def,MULT_SYM] THEN 
+ `BAG_IN e b2` by METIS_TAC [lem1] THEN
+ `?b2'. b2 = BAG_INSERT e b2'` by METIS_TAC [BAG_DECOMPOSE] THEN 
+ RW_TAC std_ss [] THEN
+ `FINITE_BAG b2'` by METIS_TAC [FINITE_BAG_THM] THEN 
+ Q.PAT_ASSUM `p = q` MP_TAC THEN RW_TAC arith_ss [BAG_GEN_PROD_REC] THEN 
+ `0 < e` by METIS_TAC [NOT_ZERO_LT_ZERO,NOT_PRIME_0] THEN 
+ FULL_SIMP_TAC arith_ss [MULT_LEFT_CANCEL] THEN POP_ASSUM (K ALL_TAC) THEN
+ `BAG_GEN_PROD b2' 1 < BAG_GEN_PROD (BAG_INSERT e b2') 1` 
+   by (RW_TAC arith_ss [BAG_GEN_PROD_REC] THEN
+       METIS_TAC [BAG_GEN_PROD_POSITIVE,BAG_IN_BAG_INSERT,NOT_ZERO_LT_ZERO,
+             NOT_PRIME_0,DECIDE``!n.(n=0) \/ (n=1) \/ 1<n``,NOT_PRIME_1]) THEN
+ `b2' = b1'` by METIS_TAC[FINITE_BAG_THM,BAG_IN_BAG_INSERT] THEN
+METIS_TAC [BAG_INSERT_ONE_ONE]]);
+
+
+val PRIME_FACTORIZATION = store_thm
+("PRIME_FACTORIZATION",
+ ``!n. 1 < n ==> 
+      !b. FINITE_BAG b /\ (!x. BAG_IN x b ==> prime x) /\
+          (BAG_GEN_PROD b 1 = n) ==> 
+      (b = PRIME_FACTORS n)``,
+ METIS_TAC [PRIME_FACTORS_def,UNIQUE_PRIME_FACTORS]);
+
+val _ = export_theory();
